code/ecdsap256/Hacl.Impl.P256.PointMul.fsti
@@ -8,90 +8,51 @@ module ST = FStar.HyperStack.ST
 open Lib.IntTypes
 open Lib.Buffer
 
-open Hacl.Spec.P256.MontgomeryMultiplication
 open Hacl.Spec.P256.Bignum
 open Hacl.Impl.P256.Point
 
 module S = Spec.P256
+module SM = Hacl.Spec.P256.MontgomeryMultiplication
 
 #set-options "--z3rlimit 30 --fuel 0 --ifuel 0"
 
 inline_for_extraction noextract
-val scalarMultiplication:
-    #buf_type:buftype
-  -> p:point
-  -> result:point
-  -> scalar:lbuffer_t buf_type uint8 (size 32)
-  -> tempBuffer:lbuffer uint64 (size 100) ->
-  Stack unit
+val scalarMultiplication: p:point -> res:point -> scalar:lbuffer uint8 32ul -> Stack unit
   (requires fun h ->
-    live h p /\ live h result /\ live h scalar /\ live h tempBuffer /\
-    LowStar.Monotonic.Buffer.all_disjoint [loc p; loc tempBuffer; loc scalar; loc result] /\
-    as_nat h (gsub p (size 0) (size 4)) < S.prime /\
-    as_nat h (gsub p (size 4) (size 4)) < S.prime /\
-    as_nat h (gsub p (size 8) (size 4)) < S.prime)
-  (ensures fun h0 _ h1 ->
-    modifies (loc p |+| loc result |+| loc tempBuffer) h0 h1 /\
-    as_nat h1 (gsub result (size 0) (size 4)) < S.prime /\
-    as_nat h1 (gsub result (size 4) (size 4)) < S.prime /\
-    as_nat h1 (gsub result (size 8) (size 4)) < S.prime /\
-    (let x3, y3, z3 = point_x_as_nat h1 result, point_y_as_nat h1 result, point_z_as_nat h1 result in
-    let (xN, yN, zN) = S.scalar_multiplication (as_seq h0 scalar) (as_point_nat h0 p) in
-    x3 == xN /\ y3 == yN /\ z3 == zN))
+    live h p /\ live h res /\ live h scalar /\
+    disjoint p res /\ disjoint scalar res /\ disjoint p scalar /\
+    point_inv h p)
+  (ensures fun h0 _ h1 -> modifies (loc p |+| loc res) h0 h1 /\
+    point_inv h1 res /\
+    as_point_nat h1 res == S.scalar_multiplication (as_seq h0 scalar) (as_point_nat h0 p))
 
 
 val scalarMultiplicationWithoutNorm:
     p:point
-  -> result:point
-  -> scalar:lbuffer uint8 (size 32)
-  -> tempBuffer: lbuffer uint64 (size 100) ->
+  -> res:point
+  -> scalar:lbuffer uint8 32ul ->
   Stack unit
   (requires fun h ->
-    live h p /\ live h result /\ live h scalar /\ live h tempBuffer /\
-    LowStar.Monotonic.Buffer.all_disjoint [loc p; loc tempBuffer; loc scalar; loc result] /\
-    as_nat h (gsub p (size 0) (size 4)) < S.prime /\
-    as_nat h (gsub p (size 4) (size 4)) < S.prime /\
-    as_nat h (gsub p (size 8) (size 4)) < S.prime)
-  (ensures fun h0 _ h1 ->
-    modifies (loc p |+| loc result |+| loc tempBuffer) h0 h1 /\
-    as_nat h1 (gsub result (size 0) (size 4)) < S.prime /\
-    as_nat h1 (gsub result (size 4) (size 4)) < S.prime /\
-    as_nat h1 (gsub result (size 8) (size 4)) < S.prime /\
-    (let p1 = fromDomainPoint(as_point_nat h1 result) in
-    let rN, _ = S.montgomery_ladder_spec (as_seq h0 scalar) ((0, 0, 0),  as_point_nat h0 p) in
-    rN == p1))
+    live h p /\ live h res /\ live h scalar /\
+    disjoint p res /\ disjoint scalar res /\ disjoint p scalar /\
+    point_inv h p)
+  (ensures fun h0 _ h1 -> modifies (loc p |+| loc res) h0 h1 /\
+    point_inv h1 res /\
+    SM.fromDomainPoint (as_point_nat h1 res) ==
+      fst (S.montgomery_ladder_spec (as_seq h0 scalar) (S.point_at_inf, as_point_nat h0 p)))
 
 
-val secretToPublic:
-    result:point
-  -> scalar:lbuffer uint8 (size 32)
-  -> tempBuffer:lbuffer uint64 (size 100) ->
-  Stack unit
+val secretToPublic: res:point -> scalar:lbuffer uint8 32ul -> Stack unit
   (requires fun h ->
-    live h result /\ live h scalar /\ live h tempBuffer /\
-    LowStar.Monotonic.Buffer.all_disjoint [loc tempBuffer; loc scalar; loc result])
-  (ensures fun h0 _ h1 ->
-    modifies (loc result |+| loc tempBuffer) h0 h1 /\
-    as_nat h1 (gsub result (size 0) (size 4)) < S.prime /\
-    as_nat h1 (gsub result (size 4) (size 4)) < S.prime /\
-    as_nat h1 (gsub result (size 8) (size 4)) < S.prime /\
-    (let x3, y3, z3 = point_x_as_nat h1 result, point_y_as_nat h1 result, point_z_as_nat h1 result in
-    let (xN, yN, zN) = S.secret_to_public (as_seq h0 scalar)  in
-    x3 == xN /\ y3 == yN /\ z3 == zN))
+    live h res /\ live h scalar /\ disjoint res scalar)
+  (ensures fun h0 _ h1 -> modifies (loc res) h0 h1 /\
+    point_inv h1 res /\ as_point_nat h1 res == S.secret_to_public (as_seq h0 scalar))
 
 
-val secretToPublicWithoutNorm:
-    result:point
-  -> scalar:lbuffer uint8 (size 32)
-  -> tempBuffer:lbuffer uint64 (size 100) ->
-  Stack unit
+val secretToPublicWithoutNorm: res:point -> scalar:lbuffer uint8 32ul -> Stack unit
   (requires fun h ->
-    live h result /\ live h scalar /\ live h tempBuffer /\
-    LowStar.Monotonic.Buffer.all_disjoint [loc tempBuffer; loc scalar; loc result])
-  (ensures fun h0 _ h1 -> modifies (loc result |+| loc tempBuffer) h0 h1 /\
-    as_nat h1 (gsub result (size 0) (size 4)) < S.prime /\
-    as_nat h1 (gsub result (size 4) (size 4)) < S.prime /\
-    as_nat h1 (gsub result (size 8) (size 4)) < S.prime /\
-    (let p1 = fromDomainPoint(as_point_nat h1 result) in
-    let rN, _ = S.montgomery_ladder_spec (as_seq h0 scalar) ((0, 0, 0), S.base_point) in
-    rN == p1))
+    live h res /\ live h scalar /\ disjoint res scalar)
+  (ensures fun h0 _ h1 -> modifies (loc res) h0 h1 /\
+    point_inv h1 res /\
+    SM.fromDomainPoint (as_point_nat h1 res) ==
+      fst (S.montgomery_ladder_spec (as_seq h0 scalar) (S.point_at_inf, S.base_point)))
