code/ecdsap256/Hacl.Impl.P256.Scalar.fst
@@ -38,7 +38,7 @@ let qmod_short_lemma a =
 [@CInline]
 let qmod_short x res =
   push_frame ();
-  let tmp = create (size 4) (u64 0) in
+  let tmp = create_felem () in
   make_order tmp;
   let h0 = ST.get () in
   let c = bn_sub4 x tmp tmp in
@@ -52,7 +52,7 @@ let qmod_short x res =
 let bn_is_lt_order_mask4 f =
   let h0 = ST.get () in
   push_frame ();
-  let tmp = create (size 4) (u64 0) in
+  let tmp = create_felem () in
   make_order tmp;
   let c = bn_sub4 f tmp tmp in
   assert (if v c = 0 then as_nat h0 f >= S.order else as_nat h0 f < S.order);
@@ -236,7 +236,7 @@ val qmont_reduction: x:widefelem -> res:felem -> Stack unit
 [@CInline]
 let qmont_reduction x res =
   push_frame ();
-  let n = create 4ul (u64 0) in
+  let n = create_felem () in
   make_order n;
 
   let h0 = ST.get () in
@@ -258,7 +258,7 @@ let qmont_reduction x res =
 let qadd x y res =
   let h0 = ST.get () in
   push_frame ();
-  let n = create 4ul (u64 0) in
+  let n = create_felem () in
   make_order n;
   bn_add_mod4 x y n res;
   let h1 = ST.get () in
@@ -270,7 +270,7 @@ let qadd x y res =
 [@CInline]
 let qmul a b res =
   push_frame ();
-  let tmp = create (size 8) (u64 0) in
+  let tmp = create_widefelem () in
   let h0 = ST.get () in
   bn_mul4 a b tmp;
   let h1 = ST.get () in
@@ -283,7 +283,7 @@ let qmul a b res =
 [@CInline]
 let fromDomainImpl a res =
   push_frame ();
-  let t = create (size 8) (u64 0) in
+  let t = create_widefelem () in
   let t_low = sub t (size 0) (size 4) in
   let t_high = sub t (size 4) (size 4) in
 
